\documentclass[10pt]{article}
\usepackage[margin=1.3cm]{geometry}

% Packages
\usepackage{amsmath, amsfonts, amssymb, amsthm}
\usepackage{bbm} 
\usepackage{dutchcal} % [dutchcal, calrsfs, pzzcal] calligraphic fonts
\usepackage{graphicx}
\usepackage[T1]{fontenc}
\usepackage[tracking]{microtype}

% Palatino for text goes well with Euler
\usepackage[sc,osf]{mathpazo}   % With old-style figures and real smallcaps.
\linespread{1.025}              % Palatino leads a little more leading

% Euler for math and numbers
\usepackage[euler-digits,small]{eulervm}

% Command initialization
\DeclareMathAlphabet{\pazocal}{OMS}{zplm}{m}{n}
\graphicspath{{./images/}}

% Custom Commands
\newcommand{\bs}[1]{\boldsymbol{#1}}
\newcommand{\E}{\mathbb{E}}
\newcommand{\var}[1]{\text{Var}\left(#1\right)}
\newcommand{\bp}[1]{\left({#1}\right)}
\newcommand{\mbb}[1]{\mathbb{#1}}
\newcommand{\1}[1]{\mathbbm{1}_{#1}}
\newcommand{\mc}[1]{\mathcal{#1}}
\newcommand{\nck}[2]{{#1\choose#2}}
\newcommand{\pc}[1]{\pazocal{#1}}
\newcommand{\ra}[1]{\renewcommand{\arraystretch}{#1}}
\newcommand*{\floor}[1]{\left\lfloor#1\right\rfloor}
\newcommand*{\ceil}[1]{\left\lceil#1\right\rceil}

\DeclareMathOperator{\Var}{Var}
\DeclareMathOperator{\Cov}{Cov}
\DeclareMathOperator{\diag}{diag}

\newtheorem{theorem}{Theorem}
\newtheorem{lemma}{Lemma}

\begin{document}

    \begin{center}
        {\bf\large{MATH 829: FUNCTIONAL ANALYSIS AND QUANTUM MECHANICS}}
        \smallskip
        \hrule
        \smallskip
        {\bf Assignment} 1\hfill {\bf Connor Braun} \hfill {\bf 2024-09-10}
    \end{center}

    \begin{center}
        \begin{minipage}{\dimexpr\paperwidth-10cm}
            {\bf ACKNOWLEDGEMENTS}\\[5pt]
            I did not collaborate with anyone on this assignment.
        \end{minipage}
    \end{center}
    \vspace{5pt}
    {\bf Problem 1} By following the steps below, prove the formula
    \begin{align}
        \lim_{n\rightarrow\infty}a_1^{(n)}=\prod_{j=2}^\infty\frac{(2j-1)^2}{4j^2-4j}=\frac{4}{\pi}\label{eq1}
    \end{align}
    where $a^{(n)}_j$ for $1\leq j\leq n$ and $n\in\mbb{N}$ are from Fourier's truncated linear system.\\[5pt]
    {\bf i)} Let $\mc{J}[n]=\int_0^\pi\sim^n(x)dx$ for $n\geq 0$. Use integration by parts to show that $\mc{J}[n]=\frac{n-1}{n}\mc{J}[n-2]$
    for $n\geq 2$. Deduce that $\tfrac{\mc{J}[2n-1]}{\mc{J}[2n+1]}=\tfrac{2n+1}{2n}$.\\[5pt]
    {\bf Solution}. As suggested, via integration by parts we obtain
    \begin{align*}
        \mc{J}[n]=\int_0^\pi\sin^n(x)dx&=-\sin^{n-1}(x)cos(x)\bigg|^\pi_0+(n-1)\int_0^\pi\cos^2(x)\sin^{n-2}(x)dx\\
        &=(n-1)\int_0^\pi(1-\sin^2(x))\sin^{n-2}(x)dx\\
        &=(n-1)\left[\int_0^\pi\sin^{n-2}(x)dx-\int_0^\pi\sin^n(x)dx\right]\\
        &=(n-1)\mc{J}[n-2]-n\mc{J}[n]+\mc{J}[n]
    \end{align*}
    whereby it is clear that $\mc{J}[n]=\tfrac{n-1}{n}\mc{J}[n-2]$. For the second claim,
    \begin{align*}
        \frac{\mc{J}[2n-1]}{\mc{J}[2n+1]}=\frac{\tfrac{2n-2}{2n-1}\mc{J}[2n-3]}{\tfrac{2n}{2n+1}\mc{J}[2n-1]}&=\frac{2n-2}{2n-1}\frac{2n+1}{2n}\frac{\mc{J}[2n-3]}{\tfrac{2n-2}{2n-1}\mc{J}[2n-3]}\\
        &=\frac{2n+1}{2n}
    \end{align*}
    as desired.\hfill{$\qed$}\\[5pt]
    {\bf ii)} Show that $1\leq \frac{\mc{J}[2n]}{\mc{J}[2n+1]}\leq\frac{2n+1}{2n}$ for $n\geq 1$ and compute $\lim_{n\rightarrow\infty}\frac{\mc{J}[2n]}{\mc{J}[2n+1]}$.\\[5pt]
    {\bf Solution}. The critical observation here is that $\forall x\in[0,\pi]$, $0\leq \sin(x)\leq 1$ such that $\sin^{n}(x)\leq \sin^{n-1}(x)$ for $n\geq 2$. This furnishes the inequality
    \begin{align*}
        \mc{J}[2n]=\int_0^\pi\sin^{2n}(x)dx\leq\int_0^\pi\sin^{2n-1}(x)dx=\mc{J}[2n-1]
    \end{align*}
    for $n\geq 1$, and in precisely the same way $\mc{J}[2n+1]\leq \mc{J}[2n]$. Thus,
    \begin{align*}
        1=\frac{\mc{J}[2n+1]}{\mc{J}[2n+1]}\leq \frac{\mc{J}[2n]}{\mc{J}[2n+1]}\leq \frac{\mc{J}[2n-1]}{\mc{J}[2n+1]}=\frac{2n+1}{2n}
    \end{align*}
    from part (i). Of course, $\lim_{n\rightarrow\infty}\tfrac{2n+1}{2n}=1$, so via the squeeze theorem, $\lim_{n\rightarrow\infty}\tfrac{\mc{J}[2n]}{\mc{J}[2n+1]}=1$.\hfill{$\qed$}\\[5pt]
    {\bf iii)} Write $\mc{J}[2n]$ and $\mc{J}[2n+1]$ as products using (i), and then use the limit from (ii) to show that 
    \[\prod_{j=1}^\infty\left(\frac{2j}{2j-1}\frac{2n}{2j+1}\right)=\frac{\pi}{2}.\]
    {\bf Solution}. Following instructions, we find that
    \begin{align*}
        \mc{J}[2n]=\frac{2n-1}{2n}\mc{J}[2n-2]=\frac{2n-1}{2n}\frac{2n-3}{2n-2}\mc{J}[2n-4]=\cdots&=\left[\prod_{j=0}^{n-1}\frac{2n-(2j+1)}{2n-2j}\right]\mc{J}[0]
    \end{align*}
    where clearly, $\mc{J}[0]=\pi$ and thus $\mc{J}[2n]=\pi \prod_{j=0}^{n-1}\tfrac{2n-(2j+1)}{2n-2j}$, for $n\geq 1$. Using the same program,
    \begin{align*}
        \mc{J}[2n+1]=\frac{2n}{2n+1}\mc{J}[2n-1]=\frac{2n}{2n+1}\frac{2n-2}{2n-1}\mc{J}[2n-3]=\cdots=\left[\prod_{j=0}^{n-1}\frac{2n+1-(2j+1)}{2n+1-2j}\right]\mc{J}[1]
    \end{align*}\
    and further $\mc{J}[1]=-\cos(x)\big|^\pi_0=2$, so $\mc{J}[2n+1]=2\prod_{j=0}^{n-1}\tfrac{2n+1-(2j+1)}{2n+1-2j}$ for $n\geq 1$. Next, form the ratio
    \begin{align*}
        \frac{\mc{J}[2n+1]}{2}\frac{\pi}{\mc{J}[2n]}=\prod_{j=0}^{n-1}\frac{2n-2j}{2n-2j+1}\frac{2n-2j}{2n-2j-1}.
    \end{align*}
    Now, define a change of variables $k=n-j$ and reverse the order of the product such that the first index is $j=n-1$ and the last is $j=0$. Then this same finite product can be realized by
    the range of indices $k=1$ to $k=n$, so
    \begin{align*}
        \frac{\pi}{2}\left(\frac{\mc{J}[2n+1]}{\mc{J}[2n]}\right)=\prod_{j=0}^{n-1}\frac{2n-2j}{2n-2j+1}\frac{2n-2j}{2n-2j-1}=\prod_{k=1}^n\frac{2k}{2k+1}\frac{2k}{2k-1}.
    \end{align*}
    Finally, taking the limit as $n\rightarrow\infty$ produces the desired result:
    \begin{align*}
        \lim_{n\rightarrow\infty}\frac{\pi}{2}\left(\frac{\mc{J}[2n+1]}{\mc{J}[2n]}\right)=\frac{\pi}{2}=\prod_{k=1}^\infty\frac{2k}{2k+1}\frac{2k}{2k-1}
    \end{align*}
    where the first equality holds by part (ii).\hfill{$\qed$}\\[5pt]
    {\bf iv)} Use (iii) to prove (\ref{eq1}).\\[5pt]
    {\bf Solution}. In part (iii) we obtained the sequence of identities
    \begin{align}
        \frac{2}{\pi}\left(\frac{\mc{J}[2n]}{\mc{J}[2n+1]}\right)=\prod_{k=1}^n\frac{2k+1}{2k}\frac{2k-1}{2k}.\label{eq2}
    \end{align} 
    for $n\geq 1$. Defining the partial product $P_n:=\prod_{j=2}^n\tfrac{(2j-1)^2}{4j^2-4j}$ for $n\geq 2$, we can manipulate (\ref{eq2}) to produce the chain of
    implications:
    \begin{align}
        (\ref{eq2})\quad\Rightarrow\quad 2\frac{3}{4}\left[\prod_{j=2}^n\frac{2j+1}{2j}\frac{2j-1}{2j}\right]=\frac{4}{\pi}\left(\frac{\mc{J}[2n]}{\mc{J}[2n+1]}\right)\quad&\Rightarrow\quad\frac{3}{2}\left[\prod_{j=2}^n\frac{(2j-1)^2}{4j^2(1-1/j)}\frac{(2j+1)(1-1/j)}{2j-1}\right]=\frac{4}{\pi}\frac{\mc{J}[2n]}{\mc{J}[2n+1]}\\
        &\Rightarrow\quad\frac{3}{2}P_n\left[\prod_{j=2}^n\frac{(2j+1)(j-1)}{j(2j-1)}\right]=\frac{4}{\pi}\frac{\mc{J}[2n]}{\mc{J}[2n+1]}.\label{eq3}
    \end{align}
    From here, take $Q_n:=\prod_{j=2}^n\tfrac{(2j+1)(j-1)}{j(2j-1)}$ and observe that this partial product has a telescopic property:
    \begin{align*}
        Q_n&=\frac{(5)(1)}{(2)(3)}\times\frac{(7)(2)}{(3)(5)}\times\frac{(9)(3)}{(4)(7)}\times\cdots\times\frac{(2n-1)(n-2)}{(n-1)(2n-3)}\frac{(2n+1)(n-1)}{(n)(2n-1)}\\
        &=\frac{1}{3}\left(\frac{2n+1}{n}\right)
    \end{align*}
    such that $Q_n\rightarrow\tfrac{2}{3}$ as $n\rightarrow\infty$. Finally, picking up at (3) and taking the limit:
    \begin{align*}
        \lim_{n\rightarrow\infty}\frac{3}{2}P_nQ_n=\lim_{n\rightarrow\infty}\frac{4}{\pi}\frac{\mc{J}[2n]}{\mc{J}[2n+1]}\quad\Rightarrow\quad \lim_{n\rightarrow\infty}P_n=\frac{4}{\pi}.
    \end{align*}
    And we are done.\hfill{$\qed$}
\end{document}